plain type as a parameter in AEAD.fsti

src/tls/AEAD.fsti
@@ -8,12 +8,19 @@ module HS = FStar.HyperStack //Added automatically
 module I = Crypto.Indexing
 module U32 = FStar.UInt32
 module U128 = FStar.UInt128
-module Plain = Crypto.Plain
+//module Plain = Crypto.Plain
 
 open FStar.Bytes
 open FStar.UInt32
 open Mem
 open Pkg
+
+
+type safeid = i:I.id{Flag.safeId i}
+type unsafeid = i:I.id{~ (Flag.safeId i)}
+
+let safeMac (i:I.id) = Flag.safeHS i && Flag.mac1 i
+let safeId  (i:I.id) = Flag.safeId i
 
 let ivlen (alg:I.cipherAlg) = 12ul
 
@@ -29,107 +36,95 @@ let aadmax =
 
 type aadlen_32 = l:U32.t {l <=^ aadmax}
 
-type info' = {
+
+
+type plainLen = l:nat{l + v taglen < pow2 32}
+
+noeq type plain_pkg =
+  | PlainPkg:
+    plain: (i:I.id -> plainLen -> eqtype) ->
+    as_bytes: (i:I.id -> l:plainLen -> plain i l -> GTot (lbytes l)) ->
+    repr: (i:unsafeid -> l:plainLen -> p:plain i l -> Tot (b:lbytes l{b == as_bytes i l p})) ->
+    plain_pkg
+
+noeq type info' = {
   alg: I.aeadAlg;
   prf_rgn: subrgn tls_tables_region;
   log_rgn: subrgn tls_tables_region;
+  plain: plain_pkg;
 }
 
 type info (i:I.id) =
   info:info'{I.aeadAlg_of_id i == info.alg}
 
+let plain (#i:I.id) (u:info i) (l:plainLen) =
+  (PlainPkg?.plain u.plain) i l
+ 
+let as_bytes (#i:I.id) (#u:info i) (#l:plainLen) (p:plain u l) : GTot (lbytes l) = 
+  (PlainPkg?.as_bytes u.plain) i l p
+  
+let repr (#i:unsafeid) (#u:info i) (#l:plainLen) (p:plain u l) : Tot (r:lbytes l{r == as_bytes p}) =
+  (PlainPkg?.repr u.plain) i l p
+
 val keylen   : #i:I.id -> u:info i -> U32.t
 
 val statelen : #i:I.id -> u:info i -> U32.t
 
-type cipher (i:I.id) (l:nat{l + v taglen < pow2 32}) = lbytes (l + (UInt32.v taglen))
+type cipher (i:I.id) (l:plainLen) = lbytes (l + (UInt32.v taglen))
 
 type cipher32 (i:I.id) (l:U32.t{UInt.size (v l + 16) 32}) = lbytes32 (l +^ taglen)
-
-inline_for_extraction
-val entry : i:I.id -> Type0
 
 type nonce (i:I.id) = iv (I.cipherAlg_of_id i)
 
 type adata = b:bytes{length b <= v aadmax}
 
-type plainLen = l:Plain.plainLen{l + v taglen < pow2 32}
+type entry (i:I.id) (u:info i) =
+  | Entry:
+    nonce: nonce i ->
+    ad: adata ->
+    #l: plainLen ->
+//    #u: info i ->
+    p: plain u l ->
+    c: cipher i l ->
+    entry i u
 
-val mk_entry (#i:I.id) :
+(*
+inline_for_extraction
+val entry : #i:I.id -> u:info i -> Type0
+
+
+val mk_entry (#i:I.id) (u:info i):
     nonce:nonce i ->
     ad:adata ->
     #l:plainLen ->
-    p:Plain.plain i l ->
-    c:cipher i (Seq.length (Plain.as_bytes p)) ->
-    entry i
+    p:plain u l ->
+    c:cipher i (length (as_bytes p)) ->
+    entry u
 
-val entry_injective (#i:I.id)
+val entry_injective (#i:I.id) (u:info i)
                     (n:nonce i) (n':nonce i)
                     (ad:adata) (ad':adata)
                     (#l:plainLen) (#l':plainLen)
-                    (p:Plain.plain i l) (p':Plain.plain i l')
-                      (c:cipher i (Seq.length (Plain.as_bytes p))) (c':cipher i (Seq.length (Plain.as_bytes p')))
-  : Lemma (let e  = mk_entry n ad p c in
-           let e' = mk_entry n' ad' p' c' in
+                    (p:plain u l) (p':plain u l')
+                    (c:cipher i l) (c':cipher i l')
+  : Lemma (let e  = mk_entry u n ad p c in
+           let e' = mk_entry u n' ad' p' c' in
            (e == e' <==> (n == n' /\ ad == ad' /\ l == l' /\ p == p' /\ c == c')))
 
-val nonce_of_entry (#i:_) (e:entry i) : nonce i
+val nonce_of_entry (#i:_) (#u:info i) (e:entry u) : nonce i
 
-val ad_of_entry (#i:_) (e:entry i) : adata
+val ad_of_entry (#i:_) (#u:info i) (e:entry u) : adata
 
-val plain_of_entry (#i:_) (e:entry i) : (l:plainLen & p:Plain.plain i l)
+val plain_of_entry (#i:_) (#u:info i) (e:entry u) : (l:plainLen & p:plain u l)
 
-let safeMac (i:I.id) = Flag.safeHS i && Flag.mac1 i
+val cipher_of_entry (#i:_) (#u:info i) (e:entry u) : cipher u
+*)
 
-let safeId  (i:I.id) = Flag.safeId i
+val aead_state: i:I.id -> I.rw -> Type0
 
-val aead_state: I.id -> I.rw -> Type0
+val getinfo: #i:I.id -> #rw:I.rw -> aead_state i rw -> Tot (info i)
 
-
-(** Draft of Stream interface & security spec
-val stream_state: I.id -> I.rw -> Type0
-
-val ctrT: #i:I.id -> #rw:_ -> wr:stream_state i rw -> mem -> GTot UInt32.t
-val log: #i:I.id -> #rw:_ -> wr:stream_state i rw -> mem -> GTot (Seq.seq (stream_entry i)
-
-val create: i:I.id -> u:info i -> rw:_
-  ST (stream_state i rw)
-  (requires fun h0 -> disjoint u.shared u.local)
-  (ensures fun h0 st h1 ->
-    I.safeId i ==>
-      (log st h1 == Seq.empty /\
-      ctrT st h1 == 0ul)
-    /\ invariant st h1
-  )
-
-val encrypt (#i:_) (w:stream_state i I.Writer) (ad:adata i) (#rg:Range.rg) (p:StreamPlain.plain l i) : ST (cipher i rg)
-  (requires fun h0 -> incrementable h0 /\ invariant h0)
-  (ensures fun h0 cipher h1 ->
-    ctrT w h1 == U32.(ctrT w h0 +^ 1ul) /\
-    invariant w h1 /\
-    I.safeId ==> (
-      (log w h1 == Seq.Cons (log w h0) (mk_entry ad p cipher))
-    /\ modifies (footprint w) h0 h1
-    ))
-
-
-val frame_invariant: #i:_ -> #rw:_ -> st:aead_state i rw -> h0:mem -> r:rid -> h1:mem ->
-    Lemma (requires (invariant st h0 /\
-           modifies_one r h0 h1 /\
-           ~(r `Set.mem` footprint st) /\
-           ~(r `Set.mem` shared_footprint)))
-          (ensures invariant st h1)
-
-val frame_log: #i:_ -> #rw:_ -> st:aead_state i rw -> l:Seq.seq (entry i) ->
-  h0:mem -> r:rid -> h1:mem ->
-
-**)
-
-val log_region: #i:_ -> #rw:_ -> aead_state i rw -> subrgn tls_tables_region
-
-val prf_region: #i:_ -> #rw:_ -> aead_state i rw -> subrgn tls_tables_region
-
-val log: #i:_ -> #rw:_ -> s:aead_state i rw{safeMac i} -> mem -> GTot (Seq.seq (entry i))
+val log: #i:I.id -> #rw:_ -> s:aead_state i rw{safeMac i} -> mem -> GTot (Seq.seq (entry i (getinfo s)))
 
 let address = nat
 
@@ -156,64 +151,58 @@ val safelen: I.id -> nat -> GTot bool
 
 let ok_plain_len_32 (i:I.id) = l:U32.t{safelen i (v l)}
 
-val invariant : #i:_ -> #rw:_ -> aead_state i rw -> mem -> Type0
+val invariant : #i:I.id -> #rw:I.rw -> aead_state i rw -> mem -> Type0
 
-val frame_invariant: #i:_ -> #rw:_ -> st:aead_state i rw -> h0:mem -> r:rid -> h1:mem ->
-    Lemma (requires (invariant st h0 /\
+val frame_invariant: #i:I.id -> #rw:I.rw -> s:aead_state i rw -> h0:mem -> r:rid -> h1:mem ->
+    Lemma (requires (invariant s h0 /\
            modifies_one r h0 h1 /\
-           ~(r `Set.mem` footprint st) /\
+           ~(r `Set.mem` footprint s) /\
            ~(r `Set.mem` shared_footprint)))
-          (ensures invariant st h1)
+          (ensures invariant s h1)
 
-val frame_log: #i:_ -> #rw:_ -> st:aead_state i rw -> l:Seq.seq (entry i) ->
+val frame_log: #i:I.id -> #rw:I.rw -> s:aead_state i rw -> l:Seq.seq (entry i (getinfo s)) ->
   h0:mem -> r:rid -> h1:mem ->
   Lemma (requires
           safeMac i /\
-          log st h0 == l /\
+          log s h0 == l /\
           modifies_one r h0 h1 /\
-          ~(r `Set.mem` footprint st))
-        (ensures log st h1 == l)
+          ~(r `Set.mem` footprint s))
+        (ensures log s h1 == l)
 
 (*** The main stateful API ***)
 
 (** Allocating a writer **)
-val gen (i:I.id)
-        (u:info i)
-  : ST (aead_state i I.Writer)
-    (requires (fun h -> u.prf_rgn `disjoint` u.log_rgn))
-    (ensures  (fun h0 s h1 ->
-               log_region s == u.log_rgn /\
-               prf_region s == u.prf_rgn /\
-               modifies_none h0 h1 /\ // allocates only
-               (exists fresh.
-                  fresh_addresses u.prf_rgn fresh h0 h1 /\
-                  footprint s == Set.singleton u.log_rgn /\
-                  shared_footprint == Set.singleton u.prf_rgn) /\
-               (safeId i ==> log s h1 == Seq.empty) /\
-               invariant s h1
-              ))
+val gen (i:I.id) (u:info i) : ST (aead_state i I.Writer)
+  (requires (fun h -> u.prf_rgn `disjoint` u.log_rgn))
+  (ensures  (fun h0 s h1 ->
+    getinfo s == u /\
+    modifies_none h0 h1 /\ // allocates only
+    (exists fresh.
+      fresh_addresses u.prf_rgn fresh h0 h1 /\
+      footprint s == Set.singleton u.log_rgn /\
+      shared_footprint == Set.singleton u.prf_rgn) /\
+      (safeId i ==> log s h1 == Seq.empty) /\
+        invariant s h1
+      ))
 
 (** Building a reader from a writer **)
 
 (* A reader never writes to the log_region, but may write to the prf_region *)
-let reader_footprint (#i:_) (wr:aead_state i I.Writer) : GTot rset =
+let reader_footprint (#i:I.id) (w:(aead_state i I.Writer)) : GTot rset =
   assume false;
-  Set.singleton (prf_region wr)
+  Set.singleton (getinfo w).prf_rgn
   
 //  TSet.filter (fun (r:HS.rid) -> r == prf_region wr)
 //                    (footprint wr)
 
-val genReader
-           (#i: I.id)
-           (wr: aead_state i I.Writer)
- : ST (aead_state i I.Reader)
-  (requires (fun h -> invariant wr h))
-  (ensures  (fun h0 rd h1 ->
-               HS.modifies Set.empty h0 h1 /\
-               invariant rd h1 /\
-               log_region rd == log_region wr /\
-               prf_region rd == prf_region wr /\
-               footprint  rd == reader_footprint wr))
+val genReader (#i: I.id) (w: aead_state i I.Writer) : ST (aead_state i I.Reader)
+  (requires (fun h -> invariant w h))
+  (ensures  (fun h0 r h1 ->
+    HS.modifies Set.empty h0 h1 /\
+    invariant r h1 /\
+    getinfo r == getinfo w /\
+    footprint r == reader_footprint w)
+  )
 
 (*
 (** [coerce]: Only needed for modeling the adversary *)
@@ -229,6 +218,7 @@ val coerce
                HS.modifies Set.empty h0 h1 /\
                invariant st h1))
 
+
 (** [leak]: Only needed for modeling the adversary *)
 val leak
       (#i: I.id)
@@ -238,6 +228,7 @@ val leak
   (ensures  (fun h0 _ h1 ->
                HS.modifies Set.empty h0 h1 /\
                invariant st h1))
+
 
 // enc_dec_separation: Calling AEAD.encrypt/decrypt requires this separation
 let enc_dec_separation (#i:_) (#rw:_) (st:aead_state i rw)
@@ -283,57 +274,60 @@ let entry_of
   let p = Plain.sel_plain h plainlen plain in
   let c = Buffer.as_seq h cipher_tag in
   mk_entry n aad p c
+*)
 
-let entry_for_nonce (#i:_) (#rw:_) (n:nonce i) (st:aead_state i rw) (h:mem{safeMac i})
-  : GTot (option (entry i)) =
-    Seq.find_l (fun e -> nonce_of_entry e = n) (log st h)
+let entry_for_nonce (#i:I.id) (#rw:I.rw) (n:nonce i) (s:aead_state i rw) (h:mem)
+  : Ghost (option (entry i (getinfo s))) (requires safeId i) (ensures fun _ -> True) =
+  Seq.find_l (fun e -> Entry?.nonce e = n) (log s h)
 
-let fresh_nonce (#i:_) (#rw:_) (n:nonce i) (st:aead_state i rw) (h:mem{safeMac i}): GTot bool =
-  None? (entry_for_nonce n st h)
+let fresh_nonce (#i:I.id) (#rw:I.rw) (n:nonce i) (s:aead_state i rw) (h:mem)
+  : Ghost bool (requires safeId i) (ensures fun _ -> True) =
+  None? (entry_for_nonce n s h)
 
-let just_one_buffer (#a:Type) (b:Buffer.buffer a) : GTot fp =
+(*let just_one_buffer (#a:Type) (b:Buffer.buffer a) : GTot fp =
    as_set [(Buffer.frameOf b, SomeRefs (as_set [Buffer.as_addr b]))]
+*)
 
 val encrypt
-          (i: I.id)
-         (st: aead_state i I.Writer)
-          (n: iv (I.cipherAlg_of_id i))
-     (aadlen: aadlen_32)
-        (aad: lbuffer (v aadlen))
-   (plainlen: ok_plain_len_32 i)
-      (plain: Plain.plainBuffer i (v plainlen))
- (cipher_tag: lbuffer (v plainlen + v taglen))
-            : ST unit
-  (requires (fun h ->
-               enc_dec_separation st aad plain cipher_tag /\
-               enc_dec_liveness st aad plain cipher_tag h /\
-               invariant st h /\
-               (safeMac i ==> fresh_nonce n st h)))
-  (ensures (fun h0 _ h1 ->
-               modifies_fp (footprint st `TSet.union` just_one_buffer cipher_tag) h0 h1 /\
-               enc_dec_liveness st aad plain cipher_tag h1 /\
-               invariant st h1 /\
-               (safeMac i ==>
-                   log st h1 ==
-                   Seq.snoc (log st h0) (entry_of n aad plain cipher_tag h1))))
+  (i: I.id)
+  (w: aead_state i I.Writer)
+  (n: iv (I.cipherAlg_of_id i))
+  (aad: adata)
+  (l: plainLen)
+  (p: plain (getinfo w) l)
+  : ST (cipher i l)
+  (requires (fun h0 ->
+//    enc_dec_separation st aad plain cipher_tag /\
+//    enc_dec_liveness st aad plain cipher_tag h /\
+    invariant w h0 /\
+    (safeId i ==> fresh_nonce n w h0)))
+  (ensures (fun h0 c h1 ->
+    modifies (Set.union (footprint w) shared_footprint) h0 h1 /\
+//    enc_dec_liveness st aad plain cipher_tag h1 /\
+    invariant w h1 /\
+    (safeId i ==>
+      log w h1 == Seq.snoc (log w h0) (Entry n aad p c))))
 
 val decrypt
-          (i: I.id)
-         (st: aead_state i I.Reader)
-          (n: iv (I.cipherAlg_of_id i))
-     (aadlen: aadlen_32)
-        (aad: lbuffer (v aadlen))
-   (plainlen: ok_plain_len_32 i)
-      (plain: Plain.plainBuffer i (v plainlen))
- (cipher_tag: lbuffer (v plainlen + v taglen))
-            : ST bool
-  (requires (fun h ->
-               enc_dec_separation st aad plain cipher_tag /\
-               enc_dec_liveness st aad plain cipher_tag h /\
-               invariant st h))
-  (ensures (fun h0 verified h1 ->
-               invariant st h1 /\
-               enc_dec_liveness st aad plain cipher_tag h1 /\
-               modifies_fp (footprint st `TSet.union` just_one_buffer (Plain.as_buffer plain)) h0 h1 /\
-               (safeId i ==> entry_for_nonce n st h1 == Some (entry_of n aad plain cipher_tag h1))))
-*)
+  (i: I.id)
+  (r: aead_state i I.Reader)
+  (aad:adata)
+  (n: iv (I.cipherAlg_of_id i))
+  (l:plainLen)
+  (c:cipher i l)
+  : ST (option (plain (getinfo r) l))
+  (requires (fun h0 ->
+    invariant r h0))
+  (ensures fun h0 res h1 ->
+    invariant r h1 /\
+    modifies (Set.union (footprint r) shared_footprint) h0 h1 /\
+    (safeId i ==>
+      (match entry_for_nonce n r h0 with
+      | None -> None? res
+      | Some (Entry _ aad' #l' p' c') ->
+        (if aad' = aad && c' = c && l = l' then res = Some p'
+        else None? res)
+      )
+    )
+  )
+
